src/CertifiedExtraction/Extraction/BasicTactics.v
@@ -15,7 +15,7 @@ Ltac compile_read value ext :=
 
 Ltac assoc_telescope tel needle :=
   match tel with (* Note that this may return None when a binding in fact exists *)
-  | Cons (Some ?k) ?v _ => let eq := constr:(eq_refl k : k = needle) in constr:(Some v)
+  | Cons (NTSome ?k) ?v _ => let eq := constr:(eq_refl k : k = needle) in constr:(Some v)
   | Cons _ _ (fun _ => ?t) => let ret := assoc_telescope t needle in constr:(ret)
   | _ => None
   end.
