src/CertifiedExtraction/Extraction/DeallocSCA.v
@@ -6,35 +6,35 @@ Lemma CompileDeallocSCA:
     {{ [[compSCA as kk]]::(tail kk)}}
       prog
     {{ [[compSCA as kk]]::(tail' kk) }} ∪ {{ ext }} // env ->
-    {{ [[k <~~ compSCA as kk]]::(tail kk)}}
+    {{ [[`k <~~ compSCA as kk]]::(tail kk)}}
       prog
     {{ [[compSCA as kk]]::(tail' kk) }} ∪ {{ ext }} // env.
 Proof.
   SameValues_Facade_t;
-  apply SameValues_Dealloc_SCA in H0;
+  learn (SameValues_Dealloc_SCA _ _ _ _ _ H0);
   SameValues_Facade_t.
 Qed.
 
-Lemma CompileDeallocSCA_ret:
-  forall {av} (env : Env av) k (v: W) tail tail' ext
-    prog,
-    {{ [[(ret v) as kk]]::(tail kk)}}
-      prog
-    {{ [[(ret v) as kk]]::(tail' kk) }} ∪ {{ ext }} // env ->
-    {{ [[k <~~ ret v as kk]]::(tail kk)}}
-      prog
-    {{ [[ret v as kk]]::(tail' kk) }} ∪ {{ ext }} // env.
-Proof.
-  intros; apply CompileDeallocSCA;
-  SameValues_Facade_t.
-Qed.
+(* Lemma CompileDeallocSCA_ret: *)
+(*   forall {av} (env : Env av) k (v: W) tail tail' ext *)
+(*     prog, *)
+(*     {{ [[(ret v) as kk]]::(tail kk)}} *)
+(*       prog *)
+(*     {{ [[(ret v) as kk]]::(tail' kk) }} ∪ {{ ext }} // env -> *)
+(*     {{ [[k <~~ ret v as kk]]::(tail kk)}} *)
+(*       prog *)
+(*     {{ [[ret v as kk]]::(tail' kk) }} ∪ {{ ext }} // env. *)
+(* Proof. *)
+(*   intros; apply CompileDeallocSCA; *)
+(*   SameValues_Facade_t. *)
+(* Qed. *)
 
 Lemma CompileDeallocSCA_discretely :
   forall {av} (tenv tenv': Telescope av) ext env k (v: W) prog,
     k ∉ ext ->
     NotInTelescope k tenv ->
-    {{ [[k <-- v as _]] :: tenv }} prog {{ [[k <-- v as _]] :: tenv' }} ∪ {{ ext }} // env ->
-    {{ [[k <-- v as _]] :: tenv }} prog {{ tenv' }} ∪ {{ ext }} // env.
+    {{ [[`k <-- v as _]] :: tenv }} prog {{ [[`k <-- v as _]] :: tenv' }} ∪ {{ ext }} // env ->
+    {{ [[`k <-- v as _]] :: tenv }} prog {{ tenv' }} ∪ {{ ext }} // env.
 Proof.
   SameValues_Facade_t.
 Qed.
